feat - basic facts about substructures

src/sub.lean
@@ -1,23 +1,168 @@
 import words
 
 namespace UA
-  universes u_lang u_str
+  universes u_lang u_str u_strA u_strB
 
   section
+
+    /- We wrap the main defenitions in a section,
+    -- so that they become universe polymorphic within this file. -/
+
+    section
+      parameter [σ : signature.{u_lang}]
+      include σ
+
+      /- a `subStructure` is a subset which is closed under the operations -/
+
+      variable {α : Type u_str}
+      variable [act : structure_on α]
+
+      @[class] def closed (sub_medium : set α) :=
+      ∀ (f) (input : vector α _), set.range input.nth ⊆ sub_medium → act f input ∈ sub_medium
+
+      def subStructure (A : Structure.{u_lang u_str}) : Type u_str :=
+      subtype (@closed A.medium A.action)
+
+    end
 
     parameter [σ : signature.{u_lang}]
     include σ
 
-    /- a `subStructure` is a subset which is closed under the operations -/
 
-    variable {α : Type u_str}
-    variable [act : structure_on α]
 
-    @[class] def closed (sub_medium : set α) :=
-    ∀ (f) (input : vector α _), set.range input.nth ⊆ sub_medium → act f input ∈ sub_medium
+    instance image_is_closed
+    {{α : Type u_strA}} {{β : Type u_strB}} [actA : structure_on α] [actB : structure_on β]
+    (φ : (α → β)) [hom : homomorphism φ] : closed (set.range φ) :=
+    begin
+      intros f yyy h,
+      rw set.range_subset_iff at h,
+      use actA f (vector.of_fn (λ i, partial_section φ ⟨yyy.nth i, h i⟩)),
+      rw ← hom _ _,
+      apply congr_arg,
+      apply vector.ext,
+      intro i,
+      rw [vector.nth_map, vector.nth_of_fn, @partial_section_prop _ _ φ _ _],
+    end
 
-    def subStructure (A : Structure.{u_lang u_str}) : Type u_str :=
-    subtype (@closed A.medium A.action)
+    lemma eval_on_substructure
+    {{α : Type u_str}} [actA : structure_on α] (X : set α) [cls : closed X] (w : word α) :
+    vars w ⊆ X → eval w ∈ X := λ h,
+    begin
+      induction w with _ f www h_ind, {
+        exact h (set.mem_singleton _),
+      },
+      {
+        apply cls f (vector.of_fn (eval ∘ www)),
+        rw set.range_subset_iff,
+        intro i,
+        rw vector.nth_of_fn,
+        rw [vars, set.Union_subset_iff] at h,
+        exact h_ind i (h i),
+      },
+    end
+
+    lemma closed_iff
+    {α : Type u_str} [actA : structure_on α] {X : set α} :
+    closed X ↔ ∀ w : word α, vars w ⊆ X → eval w ∈ X :=
+    begin
+      split, {
+        introI,
+        exact eval_on_substructure X,
+      },
+      {
+        intros h_main f xxx h,
+        convert h_main (word.opr f (word.var ∘ xxx.nth)) _, {
+          apply vector.ext,
+          intro i,
+          rw vector.nth_of_fn,
+          refl,
+        },
+        {
+          simp_rw [vars, set.Union_subset_iff, set.singleton_subset_iff],
+          rw [set.range_subset_iff] at h,
+          exact h,
+        },
+      },
+    end
+
+    def closure {{α : Type u_str}} [actA : structure_on α] (X : set α) : set α :=
+    ⋂₀ { S | closed S ∧ X ⊆ S}
+
+    instance closure_is_closed {α : Type u_str} [actA : structure_on α] {X : set α} :
+    closed (closure X) :=
+    begin
+      intros _ _ h_x S h_S,
+      apply h_S.left _ _,
+      revert h_x S,
+      rw [closure, ← set.le_eq_subset, ← set.Inf_eq_sInter],
+      exact le_Inf_iff.1,
+    end
+
+    lemma closure_inflationary {α : Type u_str} [actA : structure_on α] {X : set α} :
+    X ⊆ closure X :=
+    begin
+      intros _ _ S h_S,
+      apply h_S.right _,
+      assumption,
+    end
+
+    lemma closure_eq {α : Type u_str} [actA : structure_on α] {X : set α} :
+    closure X = eval '' {w | vars w ⊆ X} :=
+    begin
+      apply set.subset.antisymm,
+      {
+        rw [closure, ← set.le_eq_subset, ← set.Inf_eq_sInter],
+        apply Inf_le _,
+        rw set.le_eq_subset,
+        split,
+        {
+          intros f xxx h,
+          simp_rw [set.range_subset_iff, set.mem_image] at h,
+          cases choose_from_relation _ h with www h_w,
+          rw set.mem_image,
+          use word.opr f www,
+          split,
+          {
+            rw [set.mem_set_of_eq, vars, set.Union_subset_iff],
+            exact λ i, (h_w i).left,
+          },
+          {
+            convert eq.symm (UA.eval_is_hom _ (vector.of_fn www)),
+            exact funext (λ i, (eq.symm (vector.nth_of_fn _ i))),
+            apply vector.ext,
+            intro i,
+            rw [vector.nth_map, vector.nth_of_fn],
+            exact eq.symm (h_w i).right,
+          },
+        },
+        {
+          intros x h_x,
+          rw set.mem_image_eq,
+          use word.var x,
+          rw [set.mem_set_of_eq, vars],
+          exact ⟨set.singleton_subset_iff.mpr h_x, rfl⟩,
+        },
+      },
+      {
+        rw set.image_subset_iff,
+        intro w,
+        rw set.mem_preimage,
+        induction w with w f www h_ind; intro h,
+        {
+          rw [set.mem_set_of_eq, vars, set.singleton_subset_iff] at h,
+          exact closure_inflationary h,
+        },
+        {
+          refine UA.closure_is_closed f (vector.of_fn (eval ∘ www)) _,
+          rw set.range_subset_iff,
+          intro i,
+          rw vector.nth_of_fn,
+          rw [set.mem_set_of_eq, vars, set.Union_subset_iff] at h,
+          exact (h_ind i) (h i),
+        },
+      },
+    end
+
 
   end
 end UA
